Adapted depending thys to changed Collections, Refine-Monadic

thys/Tree-Automata/code/haskell/generated/Array.hs
@@ -3,26 +3,49 @@
 module Array where {
 
 
-import qualified Data.Array.Diff;
+import qualified Data.Array.Diff as Arr;
+--import qualified Data.Array as Arr;
 import Data.Array.IArray;
+import Nat;
 
-type ArrayType = Data.Array.Diff.DiffArray Int;
+instance Ix Nat where {
+    range (Nat a, Nat b) = map Nat (range (a, b));
+    index (Nat a, Nat b) (Nat c) = index (a,b) c;
+    inRange (Nat a, Nat b) (Nat c) = inRange (a, b) c;
+    rangeSize (Nat a, Nat b) = rangeSize (a, b);
+};
 
-new_array :: e -> Int -> ArrayType e;
-new_array a n = Data.Array.Diff.listArray (0, n - 1) (take n (repeat a));
+type ArrayType = Arr.DiffArray Nat;
+-- type ArrayType = Arr.Array Nat;
 
-array_length :: ArrayType e -> Int;
-array_length a = let (s, e) = bounds a in e - s + 1;
+-- we need to start at 1 and not 0, because the empty array
+-- is modelled by having s > e for (s,e) = bounds
+-- and as we are in Nat, 0 is the smallest number
 
-array_get :: ArrayType e -> Int -> e;
-array_get a i = a ! i;
+array_of_size :: Nat -> [e] -> ArrayType e;
+array_of_size n = Arr.listArray (1, n);
 
-array_set :: ArrayType e -> Int -> e -> ArrayType e;
-array_set a i e = a // [(i, e)];
+new_array :: e -> Nat -> ArrayType e;
+new_array a n = array_of_size n (repeat a);
+
+array_length :: ArrayType e -> Nat;
+array_length a = let (s, e) = bounds a in if s > e then 0 else e - s + 1;
+-- the `if` is actually needed, because in Nat we have s > e --> e - s + 1 = 1
+
+array_get :: ArrayType e -> Nat -> e;
+array_get a i = a ! (i + 1);
+
+array_set :: ArrayType e -> Nat -> e -> ArrayType e;
+array_set a i e = a // [(i + 1, e)];
 
 array_of_list :: [e] -> ArrayType e;
-array_of_list xs = Data.Array.Diff.listArray (0, length xs - 1) xs;
+array_of_list xs = array_of_size (fromInteger (toInteger (length xs - 1))) xs;
 
+array_grow :: ArrayType e -> Nat -> e -> ArrayType e;
+array_grow a i x = let (s, e) = bounds a in Arr.listArray (s, e+i) (Arr.elems a ++ repeat x);
+
+array_shrink :: ArrayType e -> Nat -> ArrayType e;
+array_shrink a sz = if sz > array_length a then undefined else array_of_size sz (Arr.elems a);
 
 
 }
