thys/Dijkstra_Shortest_Path/GraphGA.thy
@@ -1,6 +1,6 @@
 header {* Generic Algorithms for Graphs *}
 theory GraphGA
-imports GraphSpec
+imports GraphSpec "../Collections/iterator/SetIteratorOperations"
 begin
 
   definition gga_from_list :: 
@@ -10,7 +10,7 @@ begin
     where 
     "gga_from_list e a u l \<equiv> 
       let (nl,el) = l;
-        g1 = foldl (\<lambda>g v. a v g) e nl
+        g1 = foldl (\<lambda>g v. a v g) (e ()) nl
       in foldl (\<lambda>g (v,e,v'). u v e v' g) g1 el"
   
   lemma gga_from_list_correct:
@@ -28,7 +28,7 @@ begin
 
     {
       fix nl el
-      def g1\<equiv>"(foldl (\<lambda>g v. a v g) e nl)"
+      def g1\<equiv>"(foldl (\<lambda>g v. a v g) (e ()) nl)"
       def g2\<equiv>"(foldl (\<lambda>g (v,e,v'). u v e v' g) g1 el)"
       have "invar g1 \<and> \<alpha> g1 = \<lparr> nodes = set nl, edges = {} \<rparr>"
         unfolding g1_def
@@ -49,15 +49,20 @@ begin
       done
   qed
       
+  term map_iterator_product
+
   definition gga_edges_it ::
     "('V,'W,'\<sigma>,'G) graph_nodes_it \<Rightarrow> ('V,'W,'\<sigma>,'G) graph_succ_it 
     \<Rightarrow> ('V,'W,'\<sigma>,'G) graph_edges_it"
-    where
+    where "gga_edges_it ni si G \<equiv> set_iterator_product (ni G) (\<lambda>v. si G v)"
+
+(*
     "gga_edges_it ni si G c f \<sigma>0 \<equiv> 
       ni G c (
         \<lambda>v \<sigma>. si G v c (\<lambda>(w,v') \<sigma>. f (v,w,v') \<sigma>) \<sigma>
       ) \<sigma>0
     "
+*)
 
   lemma gga_edges_it_correct:
     fixes ni::"('V,'W,'\<sigma>,'G) graph_nodes_it"
@@ -70,128 +75,23 @@ begin
       graph_succ_it \<alpha> invar si by fact+
 
     show ?thesis
-    proof 
-      fix g I and \<sigma>0::'\<sigma> and c f
-      assume GI[simp, intro!]: "invar g"
-      and I0: "I (edges (\<alpha> g)) \<sigma>0"
-      and RULE: "\<And>S \<sigma> e. \<lbrakk>c \<sigma>; e\<in>S; I S \<sigma>; S\<subseteq>edges (\<alpha> g)\<rbrakk> 
-                    \<Longrightarrow> I (S-{e}) (f e \<sigma>)"
-
-      from valid[OF GI] interpret valid_graph "\<alpha> g" .
-
-      show " I {} (gga_edges_it ni si g c f \<sigma>0) \<or>
-        (\<exists>S\<subseteq>E. S \<noteq> {} \<and> \<not> c (gga_edges_it ni si g c f \<sigma>0) 
-          \<and> I S (gga_edges_it ni si g c f \<sigma>0))"
-        unfolding gga_edges_it_def
-      proof (rule_tac 
-          I="\<lambda>it \<sigma>. I (E \<inter> it\<times>UNIV\<times>UNIV) \<sigma> \<or>
-            (\<not>c \<sigma> \<and> (\<exists>S\<subseteq>E. S\<noteq>{} \<and> I S \<sigma>))
-          " 
-          in
-          set_iteratori.iterate_rule_P[OF nodes_it_correct[OF GI]])
-        
-        from E_valid have 
-          "E \<inter> V\<times>UNIV\<times>UNIV
-           = E" by auto
-        with I0 show 
-          "I (E \<inter> V\<times>UNIV\<times>UNIV) \<sigma>0 \<or> (\<not> c \<sigma>0 \<and> (\<exists>S\<subseteq>E. S\<noteq>{} \<and> I S \<sigma>0))"
-          by simp
-      next
-        fix itV \<sigma> vt
-        assume [simp, intro!]: "c \<sigma>" 
-          and [simp, intro!]: "vt\<in>itV" 
-          and IS0: "I (E \<inter> itV\<times>UNIV\<times>UNIV) \<sigma> 
-            \<or> (\<not>c \<sigma> \<and> (\<exists>S\<subseteq>E. S\<noteq>{} \<and> I S \<sigma>))"
-          and itV_SS: "itV \<subseteq> V"
-        let ?inner = "(si g vt c (\<lambda>(w, v'). f (vt, w, v')) \<sigma>)"
-        show "I (E \<inter> (itV-{vt})\<times>UNIV\<times>UNIV) ?inner \<or>
-          (\<not> c ?inner \<and> (\<exists>S\<subseteq>E. S\<noteq>{} \<and> I S ?inner))
-          "
-        proof (rule_tac I="\<lambda>itS \<sigma>. I 
-            ((E \<inter> (itV-{vt})\<times>UNIV\<times>UNIV) \<union> {vt}\<times>itS)
-            \<sigma>" in 
-          set_iteratori.iterate_rule_P[OF succ_it_correct[OF GI]])
-          have "((E \<inter> (itV-{vt})\<times>UNIV\<times>UNIV) \<union> {vt}\<times>succ (\<alpha> g) vt)
-            = (E \<inter> itV\<times>UNIV\<times>UNIV)"
-            unfolding succ_def by auto
-          with IS0 show 
-            "I ((E \<inter> (itV-{vt})\<times>UNIV\<times>UNIV) \<union> {vt}\<times>succ (\<alpha> g) vt) \<sigma>" 
-            by simp
-        next
-          fix itS \<sigma> wv
-          assume [simp, intro!]: "c \<sigma>" 
-            and [simp, intro!]: "wv\<in>itS" 
-            and "I (E \<inter> (itV - {vt}) \<times> UNIV \<times> UNIV \<union> {vt} \<times> itS) \<sigma>"
-          (is "I ?S _")
-            and itS_SS: "itS \<subseteq> succ (\<alpha> g) vt"
-
-          have "(vt,wv) \<in> ?S"
-            using itS_SS unfolding succ_def by auto
-          moreover have "?S\<subseteq>E"
-            using itS_SS unfolding succ_def by auto
-          moreover note `I ?S \<sigma>`
-          ultimately have "I (?S-{(vt,wv)}) (f (vt,wv) \<sigma>)"
-            by (auto intro!: RULE)
-          also have "(?S-{(vt,wv)}) 
-            = (E \<inter> (itV-{vt}) \<times> UNIV \<times> UNIV \<union> {vt} \<times> (itS-{wv}))"
-            by auto
-          also have "(f (vt,wv) \<sigma>) = (\<lambda>(w, v'). f (vt, w, v')) wv \<sigma>"
-            by auto
-          finally show 
-            "I (E \<inter> (itV-{vt}) \<times> UNIV \<times> UNIV \<union> {vt} \<times> (itS-{wv})) 
-               ((\<lambda>(w, v'). f (vt, w, v')) wv \<sigma>)" .
-        next
-          fix \<sigma>
-          assume "I (E \<inter> (itV - {vt}) \<times> UNIV \<times> UNIV \<union> {vt} \<times> {}) \<sigma>"
-          thus "I (E \<inter> (itV - {vt}) \<times> UNIV \<times> UNIV) \<sigma> \<or> 
-            (\<not>c \<sigma> \<and> (\<exists>S\<subseteq>E. S\<noteq>{} \<and> I S \<sigma>))"
-            by auto
-        next
-          fix \<sigma> S
-          assume "S\<subseteq>succ (\<alpha> g) vt"
-          and "S\<noteq>{}"
-          and "\<not> c \<sigma>"
-          and "I (E \<inter> (itV - {vt}) \<times> UNIV \<times> UNIV \<union> {vt} \<times> S) \<sigma>"
-          thus "I (E \<inter> (itV - {vt}) \<times> UNIV \<times> UNIV) \<sigma> \<or> 
-            (\<not>c \<sigma> \<and> (\<exists>S\<subseteq>E. S\<noteq>{} \<and> I S \<sigma>))"
-            by (auto intro!: exI[where 
-              x="(E \<inter> (itV - {vt}) \<times> UNIV \<times> UNIV \<union> {vt} \<times> S)" ]
-              simp: succ_def)
-        qed
-      next
-        fix \<sigma>
-        assume "I (edges (\<alpha> g) \<inter> {} \<times> UNIV \<times> UNIV) \<sigma> 
-          \<or> \<not> c \<sigma> \<and> (\<exists>S\<subseteq>edges (\<alpha> g). S \<noteq> {} \<and> I S \<sigma>)"
-        thus "I {} \<sigma> \<or> (\<exists>S. S \<subseteq> edges (\<alpha> g) \<and> S \<noteq> {} \<and> \<not> c \<sigma> \<and> I S \<sigma>)"
-          by auto
-      next
-        fix \<sigma> S
-        assume "S \<subseteq> nodes (\<alpha> g)" 
-          and [simp]: "S \<noteq> {}" 
-          and [simp]: "\<not> c \<sigma>"
-          and C: "I (edges (\<alpha> g) \<inter> S \<times> UNIV \<times> UNIV) \<sigma> 
-               \<or> \<not> c \<sigma> \<and> (\<exists>S\<subseteq>edges (\<alpha> g). S \<noteq> {} \<and> I S \<sigma>)"
-        from C show "I {} \<sigma> \<or> (\<exists>S. S \<subseteq> edges (\<alpha> g) \<and> S \<noteq> {} \<and> \<not> c \<sigma> \<and> I S \<sigma>)"
-        proof 
-          txt {* The case that the inner iterator was interrupted is trivial.
-            Thus, we regard the case that the outer iterator was interrupted.
-            In this case, the remaining nodes may or may not have outgoing edges.
-            In the former case, we get a proper interrupt result. In the latter
-            case, we are already finished.
-            *}
-          assume "I (edges (\<alpha> g) \<inter> S \<times> UNIV \<times> UNIV) \<sigma>"
-          thus "I {} \<sigma> \<or> (\<exists>S\<subseteq>edges (\<alpha> g). S \<noteq> {} \<and> \<not> c \<sigma> \<and> I S \<sigma>)"
-            apply (cases "(edges (\<alpha> g) \<inter> S \<times> UNIV \<times> UNIV) = {}")
-            apply simp
-            apply (rule disjI2)
-            apply (rule_tac x="(edges (\<alpha> g) \<inter> S \<times> UNIV \<times> UNIV)" in exI)
-            apply auto
-            done
-        qed simp
-      qed
+    proof
+      fix g
+      assume INV: "invar g"
+      
+      from set_iterator_product_correct[OF 
+        nodes_it_correct[OF INV] succ_it_correct[OF INV]]
+      have "set_iterator (set_iterator_product (ni g) (\<lambda>v. si g v))
+        (SIGMA v:nodes (\<alpha> g). succ (\<alpha> g) v)
+        " .
+      also have "(SIGMA v:nodes (\<alpha> g). succ (\<alpha> g) v) = edges (\<alpha> g)" 
+        unfolding succ_def 
+        by (auto dest: valid_graph.E_validD[OF valid[OF INV]])
+      finally show "set_iterator (gga_edges_it ni si g) (edges (\<alpha> g))"
+        unfolding gga_edges_it_def .
     qed
   qed
-
+        
   definition gga_to_list :: 
     "('V,'W,_,'G) graph_nodes_it \<Rightarrow> ('V,'W,_,'G) graph_edges_it \<Rightarrow> 
      ('V,'W,'G) graph_to_list"
@@ -218,11 +118,11 @@ begin
 
       have "set (ni g (\<lambda>_. True) (op #) []) = V"
         apply (rule_tac I="\<lambda>it \<sigma>. set \<sigma> = V - it" 
-          in set_iteratori.iterate_rule_P[OF nodes_it_correct])
+          in set_iterator_rule_P[OF nodes_it_correct])
         by auto
       moreover have "set (ei g (\<lambda>_. True) (op #) []) = E"
         apply (rule_tac I="\<lambda>it \<sigma>. set \<sigma> = E - it" 
-          in set_iteratori.iterate_rule_P[OF edges_it_correct])
+          in set_iterator_rule_P[OF edges_it_correct])
         by auto
       ultimately show "adjl_\<alpha> (gga_to_list ni ei g) = \<alpha> g"
         unfolding adjl_\<alpha>_def gga_to_list_def
